## Solving Quadratic Equations by Factoring

Quadratic equations are equations of the form $$ax^2 + bx + c = 0$$. When a quadratic can be factored, we can solve the equation by setting each factor equal to zero. This method uses the zero product property, which states that if $$A \times B = 0$$ then either $$A = 0$$, $$B = 0$$, or both.

### Key Concepts

- **Quadratic Equation:** An equation in the form $$ax^2 + bx + c = 0$$ where $$a \neq 0$$.

- **Factoring:** Writing the quadratic as a product of two binomials. For example, factoring $$x^2 + 5x + 6$$ gives $$(x + 2)(x + 3)$$.

- **Zero Product Property:** If $$PQ = 0$$, then at least one of $$P = 0$$ or $$Q = 0$$ must be true.

### Step-by-Step Process

1. **Write the Equation in Standard Form:**  
   Ensure the equation is in the form $$ax^2 + bx + c = 0$$. This step makes it easier to identify the coefficients for later stages.

2. **Factor the Quadratic:**  
   Find two numbers that multiply to $$a \times c$$ and add to $$b$$. These two numbers allow you to express the quadratic as a product of two binomials.

3. **Apply the Zero Product Property:**  
   Set each factor equal to zero and solve for $$x$$. This uses the principle that if a product is zero, then at least one of the factors must be zero.

4. **Check Your Solutions:**  
   Substitute your solutions into the original equation to verify that they satisfy the equation.

### Example 1: A Simple Quadratic

![Plot of $f(x)=x^2+5x+6$, showing its curve and zeros.](images/plot_1_05-01-lesson-solving-quadratic-equations-by-factoring.md.png)

Consider the quadratic equation:

$$
x^2 + 5x + 6 = 0
$$

**Step 1:**  
The equation is already in standard form.

**Step 2:**  
Factor the quadratic. Since $$a=1$$, we look for two numbers that multiply to $$6$$ (because $$1 \times 6 = 6$$) and add to $$5$$. These numbers are $$2$$ and $$3$$. Thus, the equation factors as:

$$
(x + 2)(x + 3) = 0
$$

**Step 3:**  
Apply the zero product property by setting each factor equal to zero:

$$
x + 2 = 0 \quad \text{or} \quad x + 3 = 0
$$

Solving these gives:

$$
x = -2 \quad \text{or} \quad x = -3
$$

**Result:**  
The solutions are $$x = -2$$ and $$x = -3$$. This example shows how breaking the quadratic into factors simplifies the process of finding its solutions.

### Example 2: Quadratic with Leading Coefficient Greater Than 1

Solve the equation:

$$
2x^2 + 7x + 3 = 0
$$

**Step 1:**  
The equation is in standard form.

**Step 2:**  
Calculate $$a \times c = 2 \times 3 = 6$$. Look for two numbers that multiply to $$6$$ and add to $$7$$; these numbers are $$6$$ and $$1$$. Rewrite the middle term using these numbers:

$$
2x^2 + 6x + x + 3 = 0
$$

Group the terms:

$$
(2x^2 + 6x) + (x + 3) = 0
$$

Factor out the common factors in each group:

$$
2x(x + 3) + 1(x + 3) = 0
$$

Factor by grouping:

$$
(x + 3)(2x + 1) = 0
$$

**Step 3:**  
Set each factor equal to zero:

$$
x + 3 = 0 \quad \text{or} \quad 2x + 1 = 0
$$

Solve for $$x$$:

$$
x = -3 \quad \text{or} \quad 2x = -1 \quad \Rightarrow \quad x = -\frac{1}{2}
$$

**Result:**  
The solutions are $$x = -3$$ and $$x = -\frac{1}{2}$$. This example shows the additional steps required when the leading coefficient is greater than 1, emphasizing the usefulness of the grouping method.

### Real-World Application

Imagine you are designing a rectangular garden and need to determine possible dimensions. A quadratic equation may arise when setting up design constraints. If the factored form of the equation shows one factor equaling zero, it might indicate an impractical dimension (such as a length of zero). Factoring the quadratic reveals such critical breakpoints, guiding you in adjusting your design to ensure all dimensions are viable.

> Understanding the factoring process and the zero product property builds an intuitive sense for solving quadratic equations. Recognizing that each factor contributes to the overall solution can reinforce your problem-solving skills and prepare you for more advanced algebraic techniques.